# Background
### VLB Bound
$\begin{align}
& \mathbb{E}_{q(\mathbf{x}_0)}[-\log p_{\theta}(\mathbf{x}_0)] \\ 
&= -\mathbb{E}_{q(\mathbf{x}_0)}[\log (p_{\theta}(\mathbf{x}_0) \int p_{\theta} (\mathbf{x}_{1:T})d\mathbf{x}_{1:T})] \\
&= -\mathbb{E}_{q(\mathbf{x}_0)}[ \log(\int p_{\theta} (\mathbf{x}_{0:T})d\mathbf{x}_{1:T})] \\
&= -\mathbb{E}_{q(\mathbf{x}_0)}[\log (\int q (\mathbf{x}_{1:T}|\mathbf{x}_0) \frac{ p_{\theta} (\mathbf{x}_{0:T}) }{q(\mathbf{x}_{1:T}|\mathbf{x}_0) }d\mathbf{x}_{1:T}] \\
&= -\mathbb{E}_{q(\mathbf{x}_0)}[\log (E_{ q (\mathbf{x}_{1:T}|\mathbf{x}_0)} \frac{ p_{\theta} (\mathbf{x}_{0:T}) }{q(\mathbf{x}_{1:T}|\mathbf{x}_0) })] \\
&\leq -\mathbb{E}_{q(\mathbf{x}_{0:T})}[\log \frac{ p_{\theta} (\mathbf{x}_{0:T}) }{q(\mathbf{x}_{1:T}|\mathbf{x}_0) })] = L_{VLB}
\end{align}$
$\begin{align}
L_{VLB} &= \mathbb{E_q}[-\log \frac{p_{\theta}(\mathbf{x}_{0:T})}{q(\mathbf{x}_{1:T}|\mathbf{x}_0)})]
\\ &= \mathbb{E_q}[-\log p(\mathbf{x}_T)- \sum_{t \geq 1}\log \frac{p_{\theta}(\mathbf{x}_{t-1}|\mathbf{x}_t)}{q(\mathbf{x}_{t}|\mathbf{x}_{t-1})})]
\\ &= \mathbb{E_q}[-\log p(\mathbf{x}_T)- \sum_{t >1}\log \frac{p_{\theta}(\mathbf{x}_{t-1}|\mathbf{x}_t)}{q(\mathbf{x}_{t}|\mathbf{x}_{t-1})}) - \log \frac{p_{\theta}(\mathbf{x}_{0}|\mathbf{x}_1)}{q(\mathbf{x}_{1}|\mathbf{x}_{0})}] 
\\ &= \mathbb{E_q}[-\log p(\mathbf{x}_T)- \sum_{t >1}\log \frac{p_{\theta}(\mathbf{x}_{t-1}|\mathbf{x}_t)}{q(\mathbf{x}_{t-1}|\mathbf{x}_{t}, \mathbf{x}_0)}\frac{q(\mathbf{x}_{t-1}|\mathbf{x}_0)}{q(\mathbf{x}_t|\mathbf{x}_0)}) - \log \frac{p_{\theta}(\mathbf{x}_{0}|\mathbf{x}_1)}{q(\mathbf{x}_{1}|\mathbf{x}_{0})}] 
\\ &= \mathbb{E_q}[-\log \frac{p(\mathbf{x}_T)}{q(\mathbf{x}_T|\mathbf{x}_0)}- \sum_{t >1}\log \frac{p_{\theta}(\mathbf{x}_{t-1}|\mathbf{x}_t)}{q(\mathbf{x}_{t-1}|\mathbf{x}_{t}, \mathbf{x}_0)} - \log p_{\theta}(\mathbf{x}_{0}|\mathbf{x}_1)]
\\ &= \mathbb{E_q}[ D_{\text{KL}}(q(\mathbf{x}_T|\mathbf{x}_0)||p_(\mathbf{x}_T)) + \sum_{t>1} D_{\text{KL}}(q(\mathbf{x}_{t-1}|\mathbf{x}_t, \mathbf{x}_0)||p_{\theta}(\mathbf{x}_{t-1}|\mathbf{x}_t))-\log p_{\theta}(\mathbf{x}_{0}|\mathbf{x}_1)]
\end{align}$
### Some Distributions

- $q(x_t|x_{t-1}):= \mathcal{N}(x_t; \sqrt{1-\beta_t}x_{t-1}, \sqrt{\beta_t}\mathbf{I})$
- $q(x_t|x_0) \sim \mathcal{N} (x_t; \sqrt{\bar{\alpha}_t}x_0, (1 - \bar{\alpha}_t) \mathbf{I})$
   - Let $\alpha_t = 1 - \beta_t$, $\bar{\alpha}_t = \alpha_1 \alpha_2 \cdots \alpha_t$
   - $\begin{align}
x_t &= \sqrt{\alpha_t} x_{t-1} + \sqrt{1-\alpha_t} \epsilon_1 \\
&= \sqrt{\alpha_t \alpha_{t-1}} x_{t-2} + \sqrt{1-\alpha_t} \epsilon_t + \sqrt{\alpha_t - \alpha_t \alpha_{t-1}} \epsilon_{2} \\
&=\sqrt{\alpha_t \alpha_{t-1}}x_{t-2} + \sqrt{1-\alpha_t \alpha_{t-1}} \bar{\epsilon}_{2} \\
&= \sqrt{\alpha_t \alpha_{t-1} \cdots \alpha_1}x_{0} + \sqrt{1-\alpha_t \alpha_{t-1}\cdots \alpha_0} \bar{\epsilon}_{t} \\
&:= \sqrt{\bar{\alpha_t}} x_0 + \sqrt{1-\bar{\alpha_t}} \bar{\epsilon}_t
\end{align}$
- $q(x_{t-1}|x_t, x_0) \sim \mathcal{N} (x_{t-1}; \tilde{\mu}_t (x_t, x_0), \tilde{\beta}_t \mathbf{I})$
   - ![image.png](https://cdn.nlark.com/yuque/0/2023/png/27584564/1697757475267-c1edbc41-caec-4570-8222-e847dd71ba0e.png#averageHue=%23f3f3f3&clientId=u961053e4-f864-4&from=paste&height=76&id=ud33762e7&originHeight=151&originWidth=1186&originalType=binary&ratio=2&rotation=0&showTitle=false&size=37498&status=done&style=none&taskId=u289fa311-77ef-4b37-b8a5-13700311a7d&title=&width=593)
- ![image.png](https://cdn.nlark.com/yuque/0/2023/png/27584564/1697761841777-375e6f5a-04a6-4647-bf0e-780553b06691.png#averageHue=%23f4f4f4&clientId=u2c57025a-ea68-4&from=paste&height=482&id=ua2c47993&originHeight=963&originWidth=1087&originalType=binary&ratio=2&rotation=0&showTitle=false&size=201395&status=done&style=none&taskId=ufa5fa872-e83b-49ef-8aa1-1a830216d41&title=&width=543.5)
- KL divergence of two Gaussian: $D_{KL}(P \| Q) = \log\left(\frac{\sigma_Q}{\sigma_P}\right) + \frac{\sigma_P^2 + (\mu_P - \mu_Q)^2}{2\sigma_Q^2} - \frac{1}{2}$
# Reverse process

- $p_{\theta}(\mathbf{x}_{t-1} |\mathbf{x}_t) = \mathcal{N}(\mathbf{x}_{t-1}; \boldsymbol{\mu}_{\theta}(\mathbf{x}_t, t), \boldsymbol{\Sigma}_{\theta}(\mathbf{x}_t, t))$for $1 \leq t \leq T$
- We set$\boldsymbol{\Sigma}_{\theta}(x_t, t) = \sigma_t^2 \mathbf{I}$. Experimentally, both $\sigma_t^2 = \beta_t$and $\sigma_t^2 = \tilde{\beta}_t = \frac{1 - \bar{\alpha}_{t-1}}{1 - \bar{\alpha}_t} \beta_t$ had similar results
   - Q: In the reverse, why we set$\boldsymbol{\Sigma}_{\theta}(x_t, t)$to be independent of $x_t$



